bfs example

Set_Graphs/Graph_Algorithms/BFS_Example.thy
@@ -1,6 +1,346 @@
 theory BFS_Example
-  imports BFS_2"HOL-Data_Structures.RBT_Map" Set2_Join_RBT
+  imports BFS_2 "HOL-Data_Structures.RBT_Map" Set2_Join_RBT
 begin
+
+locale BFS_subprocedures =
+  Graph: Pair_Graph_Specs
+    where lookup = lookup +
+  set_ops: Set2 neighb_empty neighb_delete _ t_set neighb_inv insert
+  
+for lookup :: "'adj \<Rightarrow> 'ver \<Rightarrow> 'neighb option" +
+
+fixes G::"'adj" 
+fixes fold_neighb::"('ver \<Rightarrow> 'neighb \<Rightarrow> 'neighb) \<Rightarrow> 'neighb \<Rightarrow> 'neighb \<Rightarrow> 'neighb"
+fixes fold_adj::"('ver \<Rightarrow> 'adj \<Rightarrow> 'adj) \<Rightarrow> 'neighb \<Rightarrow> 'adj \<Rightarrow> 'adj"
+assumes fold_neighb:"\<And> N f acc. neighb_inv N \<Longrightarrow> \<exists> xs. set xs = t_set N \<and>
+                        fold_neighb f N acc = foldr f xs acc"
+assumes fold_adj:"\<And> N f acc. neighb_inv N \<Longrightarrow> \<exists> xs. set xs = t_set N \<and>
+                        fold_adj f N acc = foldr f xs acc"
+
+begin
+
+definition next_frontier::"'neighb \<Rightarrow> 'neighb \<Rightarrow> 'neighb"  where
+"next_frontier frontier vis= fold_neighb (\<lambda> u nf. case (lookup G u) of None \<Rightarrow> nf
+                                                  | Some vs \<Rightarrow> union nf (diff vs vis)) frontier neighb_empty"
+
+lemma next_frontier:
+    "\<lbrakk>neighb_inv frontier; neighb_inv vis; Graph.graph_inv G\<rbrakk> \<Longrightarrow>  neighb_inv (next_frontier frontier vis)"
+    "\<lbrakk>neighb_inv frontier; neighb_inv vis; Graph.graph_inv G\<rbrakk> \<Longrightarrow>
+       t_set (next_frontier frontier vis) =
+         (\<Union> {Pair_Graph.neighbourhood (Graph.digraph_abs G) u | u . u \<in> t_set frontier}) - t_set vis"
+proof-
+  assume assms: "neighb_inv frontier" "neighb_inv vis" "Graph.graph_inv G"
+  obtain xs where xs_prop:True
+       "set xs = [frontier]\<^sub>s"
+       "next_frontier frontier vis =
+        foldr (\<lambda>u nf. case lookup G u of None \<Rightarrow> nf | Some vs \<Rightarrow> nf \<union>\<^sub>G (vs -\<^sub>G vis)) xs \<emptyset>\<^sub>N"
+    using fold_neighb[OF assms(1)] by(fastforce simp add: next_frontier_def)
+  have goal1_gen:"neighb_inv (foldr (\<lambda>u nf. case lookup G u of None \<Rightarrow> nf | Some vs \<Rightarrow> nf \<union>\<^sub>G (vs -\<^sub>G vis)) xs \<emptyset>\<^sub>N)" for xs
+   using assms 
+    by (induction xs)(auto split: option.split intro!: Graph.neighb.set.invar_empty set_ops.invar_union Cons set_ops.invar_diff)
+  thus"neighb_inv (next_frontier frontier vis)"
+   by(simp add: xs_prop(3)) 
+  show "[next_frontier frontier vis]\<^sub>s = \<Union> {neighbourhood [G]\<^sub>g u |u. u \<in> [frontier]\<^sub>s} - [vis]\<^sub>s"
+    unfolding xs_prop(3) 
+    using xs_prop(1,2) assms(1) 
+  proof(induction xs arbitrary: frontier)
+    case Nil
+    then show ?case by(auto intro!: Graph.neighb.set.set_empty)
+  next
+    case (Cons a xs)
+    show ?case 
+    proof(cases "a \<in> set xs")
+      case True
+      show ?thesis 
+      proof(cases "lookup G a")
+        case None
+        then show ?thesis 
+          using True Cons(2-) by (simp, intro Cons(1)) auto
+      next
+        case (Some vs)
+        have vs_already_in:"[vs]\<^sub>s 
+             \<subseteq>  \<Union> {neighbourhood [G]\<^sub>g u |u. u \<in> [frontier]\<^sub>s}"
+          using  Cons.prems(2) True Some insert_absorb 
+          by (fastforce simp add:  Graph.neighbourhood_abs[OF assms(3), symmetric] Graph.neighbourhood_def)   
+        have helper: " \<Union> {neighbourhood [G]\<^sub>g u |u. u \<in> [frontier]\<^sub>s} - [vis]\<^sub>s \<union> [vs -\<^sub>G vis]\<^sub>s =
+         \<Union> {neighbourhood [G]\<^sub>g u |u. u \<in> [frontier]\<^sub>s} - [vis]\<^sub>s"
+          using assms  vs_already_in  Some
+          by (subst set_ops.set_diff)(auto intro: set_ops.invar_diff)
+        have hlper2: "[foldr (\<lambda>u nf. case lookup G u of None \<Rightarrow> nf | Some vs \<Rightarrow> nf \<union>\<^sub>G (vs -\<^sub>G vis)) xs \<emptyset>\<^sub>N]\<^sub>s \<union> [vs -\<^sub>G vis]\<^sub>s =
+    \<Union> {neighbourhood [G]\<^sub>g u |u. u \<in> [frontier]\<^sub>s} - [vis]\<^sub>s"
+          using True Cons(2-) helper by (subst Cons(1)) auto
+        from Some show ?thesis
+          using assms(2) assms(3)  hlper2 
+          by (simp, subst set_ops.set_union)(auto intro: set_ops.invar_diff  goal1_gen)
+      qed
+    next
+      case False
+      thus ?thesis
+    proof(cases "lookup G a")
+      case None
+      hence same_neighbs:"\<Union> {neighbourhood [G]\<^sub>g u |u. u \<in> [frontier]\<^sub>s} =
+            \<Union> {neighbourhood [G]\<^sub>g u |u. u \<in> [neighb_delete a frontier]\<^sub>s}"
+          using  Graph.neighb.set.set_delete[OF Cons(4)] Graph.neighb.set.set_empty  Graph.neighb.set.set_isin[OF  Graph.neighb.set.invar_empty]
+                 neighbourhoodI 
+          by(fastforce simp add: Graph.neighb.set.set_delete[OF Cons.prems(3)] Graph.digraph_abs_def Graph.neighbourhood_def)
+     have "[foldr (\<lambda>u nf. case lookup G u of None \<Rightarrow> nf | Some vs \<Rightarrow> nf \<union>\<^sub>G (vs -\<^sub>G vis)) xs \<emptyset>\<^sub>N]\<^sub>s =
+         \<Union> {neighbourhood [G]\<^sub>g u |u. u \<in> [neighb_delete a frontier]\<^sub>s} - [vis]\<^sub>s"
+          using Cons(2-4)  Graph.neighb.set.set_delete 
+          by (intro Cons(1))(auto simp add: Graph.neighb.set.invar_delete False)+
+        thus ?thesis by (simp add: None same_neighbs)
+    next
+      case (Some vs)
+      have same_neighbs:"\<Union> {neighbourhood [G]\<^sub>g u |u. u \<in> [frontier]\<^sub>s} =
+            \<Union> {neighbourhood [G]\<^sub>g u |u. u \<in> [neighb_delete a frontier]\<^sub>s} \<union> [vs]\<^sub>s"
+      proof(rule, all \<open>rule\<close>, goal_cases)
+        case (1 x)
+        then obtain u where u_prop:"x \<in> neighbourhood [G]\<^sub>g u" "u \<in> [frontier]\<^sub>s" by auto
+        show ?case 
+        proof(cases "u = a")
+          case True
+          hence "x \<in> [vs]\<^sub>s"
+            using u_prop Some Graph.neighb.set.set_isin assms(3) 
+            by(auto split: option.split simp add: neighbourhood_def Graph.digraph_abs_def Graph.neighbourhood_def)
+          then show ?thesis  by simp
+        next
+          case False
+          hence "u \<in> [neighb_delete a frontier]\<^sub>s"
+            by (simp add: Cons.prems(3) Graph.neighb.set.set_delete u_prop(2))
+          thus ?thesis 
+            using u_prop(1) by auto
+        qed
+      next
+        case (2 x)
+        note 22 =this
+        show ?case 
+        proof(cases rule: UnE[OF 2])
+          case 1
+          then obtain u where "x \<in> neighbourhood [G]\<^sub>g u" "u \<in> [neighb_delete a frontier]\<^sub>s" by auto
+          moreover hence "u \<in> [frontier]\<^sub>s"
+            by (simp add: Cons.prems(3) Graph.neighb.set.set_delete)
+          ultimately show ?thesis by auto
+        next
+          case 2
+          hence "x \<in> neighbourhood [G]\<^sub>g a" 
+            using  Graph.neighbourhood_abs[OF assms(3)] Graph.neighbourhood_def Some by fastforce
+          moreover have "a  \<in> [frontier]\<^sub>s"
+            using Cons.prems(2) by auto
+          ultimately show ?thesis by auto
+        qed
+      qed
+      have diff_sol: "[vs -\<^sub>G vis]\<^sub>s = [vs]\<^sub>s - [vis]\<^sub>s"
+        using Some assms(2) 
+        by(auto intro: Graph.graph_invE[OF assms(3)]  simp add: set_ops.set_diff)
+      have IH_applied: "[foldr (\<lambda>u nf. case lookup G u of None \<Rightarrow> nf | Some vs \<Rightarrow> nf \<union>\<^sub>G (vs -\<^sub>G vis)) xs \<emptyset>\<^sub>N]\<^sub>s =
+                   \<Union> {neighbourhood [G]\<^sub>g u |u. u \<in> [neighb_delete a frontier]\<^sub>s} - [vis]\<^sub>s"
+        using Cons.prems(1)  Cons.prems(2)
+        by(intro  Cons(1)[of "neighb_delete a frontier"])
+          (auto simp add: False Cons.prems(3) Graph.neighb.set.invar_delete Graph.neighb.set.set_delete[OF  Cons.prems(3)] )
+      show ?thesis 
+        using Some assms(2) assms(3)  
+        by (simp add: Some same_neighbs Un_Diff, subst set_ops.set_union)
+           (auto intro: goal1_gen set_ops.invar_diff simp add: diff_sol IH_applied)
+      qed
+    qed
+  qed
+qed
+
+definition expand_tree::"'adj \<Rightarrow> 'neighb \<Rightarrow> 'neighb \<Rightarrow> 'adj" where
+"expand_tree BFS_tree frontier vis = 
+fold_adj (\<lambda> u nf. case (lookup G u) of None \<Rightarrow> nf
+                | Some vs \<Rightarrow> (case (lookup nf u) of None \<Rightarrow> update u (diff vs vis) nf
+                              | Some vs' \<Rightarrow>update u (union vs' (diff vs vis)) nf)) frontier BFS_tree"
+
+lemma expand_tree:
+     "\<lbrakk>Graph.graph_inv BFS_tree; neighb_inv frontier; neighb_inv vis; Graph.graph_inv G\<rbrakk> \<Longrightarrow> 
+       Graph.graph_inv (expand_tree BFS_tree frontier vis)"
+     "\<lbrakk>Graph.graph_inv BFS_tree; neighb_inv frontier; neighb_inv vis; Graph.graph_inv G\<rbrakk> \<Longrightarrow>
+        Graph.digraph_abs (expand_tree BFS_tree frontier vis) = 
+         (Graph.digraph_abs BFS_tree) \<union> 
+         {(u,v) | u v. u \<in> t_set (frontier) \<and> 
+                       v \<in> (Pair_Graph.neighbourhood (Graph.digraph_abs G) u -
+                       t_set vis)}"
+proof-
+  assume assms: "Graph.graph_inv BFS_tree" "neighb_inv frontier" "neighb_inv vis" "Graph.graph_inv G"
+  define one_it where "one_it = (\<lambda>u nf.
+          case lookup G u of None \<Rightarrow> nf
+          | Some vs \<Rightarrow>
+              case lookup nf u of None \<Rightarrow> update u (vs -\<^sub>G vis) nf
+              | Some vs' \<Rightarrow> update u (vs' \<union>\<^sub>G (vs -\<^sub>G vis)) nf)"
+  obtain xs where xs_prop:
+    "set xs = [frontier]\<^sub>s" "expand_tree BFS_tree frontier vis = foldr one_it xs BFS_tree"
+    using fold_adj[OF assms(2), of _ BFS_tree]
+    by (auto simp add: expand_tree_def one_it_def)
+  have goal1_general:"Graph.graph_inv (foldr one_it xs BFS_tree)" for xs
+  proof(induction xs)
+    case Nil
+    then show ?case using assms(1) by simp
+  next
+    case (Cons a xs)
+    have helper1: "\<And>v neighb.
+       lookup (foldr one_it xs BFS_tree) a = None \<Longrightarrow>
+       lookup G a = Some x2 \<Longrightarrow>
+       (if v = a then Some (x2 -\<^sub>G vis) else lookup (foldr one_it xs BFS_tree) v) = Some neighb \<Longrightarrow>
+       neighb_inv neighb" for x2 
+      by (metis Graph.graph_invE assms(3) assms(4) local.Cons option.inject set_ops.invar_diff)
+    have helper2: "lookup (foldr one_it xs BFS_tree) a = None \<Longrightarrow>
+          lookup G a = Some x2 \<Longrightarrow> Graph.graph_inv (update a (x2 -\<^sub>G vis) (foldr one_it xs BFS_tree))"
+      for x2
+      by(auto simp add: Graph.graph_inv_def Cons[simplified  Graph.graph_inv_def]  Graph.adj.map_update intro!: Graph.adj.invar_update helper1)
+    have helper3: "lookup (foldr one_it xs BFS_tree) a = Some x2a \<Longrightarrow>
+       lookup G a = Some x2 \<Longrightarrow>
+       lookup (update a (x2a \<union>\<^sub>G (x2 -\<^sub>G vis)) (foldr one_it xs BFS_tree)) v = Some neighb \<Longrightarrow> neighb_inv neighb"
+      for x2 x2a v neighb
+      apply(rule Graph.graph_invE[OF Cons] )
+      apply(rule Graph.graph_invE[OF assms(4)] )
+      apply(subst (asm)  Graph.adj.map_update) 
+      by(simp, rule  case_split[of "v = a"], auto simp add:  assms(3) assms(4) Cons  set_ops.invar_diff set_ops.invar_union)
+    have helper4:"lookup (foldr one_it xs BFS_tree) a = Some x2a \<Longrightarrow>
+       lookup G a = Some x2 \<Longrightarrow> Graph.graph_inv (update a (x2a \<union>\<^sub>G (x2 -\<^sub>G vis)) (foldr one_it xs BFS_tree))"
+      for x2 x2a
+      using Graph.adj.invar_update local.Cons 
+      by(auto intro: helper3 simp add:  Graph.graph_inv_def Cons[simplified  Graph.graph_inv_def])
+    show ?case 
+      using Cons 
+      by(simp, subst one_it_def)(auto intro: helper2 helper4 split: option.split )
+  qed
+  thus " Graph.graph_inv (expand_tree BFS_tree frontier vis)"
+    by (simp add: xs_prop(2))
+  have one_it_graph_abs:"Graph.graph_inv T \<Longrightarrow> [one_it u T]\<^sub>g = [T]\<^sub>g \<union> {(u, v) |v. v \<in> neighbourhood [G]\<^sub>g u - [vis]\<^sub>s}" for u T
+  proof(goal_cases)
+    case 1
+    note one=this
+    show ?case
+    proof(cases "lookup G u")
+      case None
+      then show ?thesis 
+        using  Graph.neighb.emptyD(1) 
+        by(simp add: one_it_def Graph.neighbourhood_abs[OF assms(4), symmetric] Graph.neighbourhood_def) 
+    next
+      case (Some vs)
+      note some=this
+      hence vs_inv:"neighb_inv vs" 
+        using assms(4) by auto
+      show ?thesis 
+      proof(cases "lookup T u")
+        case None
+        have helper:"{(ua, v). v \<in>\<^sub>G (case lookup (update u (vs -\<^sub>G vis) T) ua of None \<Rightarrow> \<emptyset>\<^sub>N | Some neighb \<Rightarrow> neighb)} =
+    {(u, v). v \<in>\<^sub>G (case lookup T u of None \<Rightarrow> \<emptyset>\<^sub>N | Some neighb \<Rightarrow> neighb)} \<union>
+    {(u, v) |v. v \<in>\<^sub>G vs \<and> v \<notin> [vis]\<^sub>s}"
+        proof(rule, all \<open>rule\<close>, goal_cases)
+          case (1 e)
+          then obtain x y where xy_prop: "e = (x,y)" 
+              "y \<in>\<^sub>G (case lookup (update u (vs -\<^sub>G vis) T) x of None \<Rightarrow> \<emptyset>\<^sub>N | Some neighb \<Rightarrow> neighb)"
+            by auto
+          then show ?case
+            using one 
+            by (subst (asm) Graph.adj.map_update) (auto intro: case_split[of "u = x"]split: option.split simp add: Graph.neighb.set.set_isin vs_inv assms(3) set_ops.invar_diff set_ops.set_diff)
+        next
+          case (2 e)
+          show ?case 
+          proof(cases rule: UnE[OF 2])
+            case 1
+            then obtain x y where "e = (x,y)" "y \<in>\<^sub>G (case lookup T x of None \<Rightarrow> \<emptyset>\<^sub>N | Some neighb \<Rightarrow> neighb)" by auto
+            then show ?thesis 
+              using one 
+              by (subst Graph.adj.map_update)(auto simp add: Graph.neighb.set.invar_empty Graph.neighb.set.set_empty Graph.neighb.set.set_isin None)
+          next
+            case 2
+            then obtain y where "e = (u,y)" "y \<in>\<^sub>G vs \<and> y \<notin> [vis]\<^sub>s" by auto
+            then show ?thesis
+              using one 
+              by (subst Graph.adj.map_update)(auto simp add: Graph.neighb.set.set_isin assms(3) set_ops.invar_diff set_ops.set_diff vs_inv)
+          qed
+        qed 
+        show ?thesis
+          using helper 
+          by(auto simp add: one_it_def None Graph.digraph_abs_def Graph.neighbourhood_def some neighbourhood_def split: option.split)
+      next
+        case (Some vs')
+        have "{(ua, y).
+     isin (case lookup (update u (vs' \<union>\<^sub>G (vs -\<^sub>G vis)) T) ua of None \<Rightarrow> \<emptyset>\<^sub>N | Some neighb \<Rightarrow> neighb) y} =
+    {(u, y). isin (case lookup T u of None \<Rightarrow> \<emptyset>\<^sub>N | Some neighb \<Rightarrow> neighb) y} \<union>
+    {(u, v) |v. v \<in>\<^sub>G vs \<and> v \<notin> [vis]\<^sub>s}"
+        proof(rule, all\<open>rule\<close>, goal_cases)
+          case (1 e)
+           then obtain x y where "e= (x,y)" "y \<in>\<^sub>G (case lookup (update u (vs' \<union>\<^sub>G (vs -\<^sub>G vis)) T) x of None \<Rightarrow> \<emptyset>\<^sub>N | Some neighb \<Rightarrow> neighb)"
+             by blast
+           thus ?case
+             apply(subst (asm) Graph.adj.map_update)
+             using one apply fast
+             using Graph.neighb.set.set_isin Some assms(3) one set_ops.invar_diff 
+             set_ops.invar_union set_ops.set_diff set_ops.set_union vs_inv  
+             by(cases "u = x", all \<open>cases "lookup T x"\<close>) auto
+         next
+           case (2 e)
+           show ?case
+           proof(cases rule: UnE[OF 2])
+             case 1
+             then obtain x y where "e = (x,y)" "y \<in>\<^sub>G (case lookup T x of None \<Rightarrow> \<emptyset>\<^sub>N | Some neighb \<Rightarrow> neighb)"
+               by auto
+             moreover hence "lookup T x \<noteq> None" 
+               using Graph.neighb.set.invar_empty Graph.neighb.set.set_empty Graph.neighb.set.set_isin by fastforce
+            ultimately show ?thesis 
+              using Graph.neighb.set.set_isin Some assms(3) 
+                    one set_ops.invar_diff set_ops.invar_union set_ops.set_union vs_inv 
+              by (subst  Graph.adj.map_update) auto
+          next
+            case 2
+            thus ?thesis
+              using Graph.neighb.set.set_isin Some assms(3) one set_ops.invar_diff 
+                    set_ops.invar_union set_ops.set_diff set_ops.set_union vs_inv 
+              by (subst  Graph.adj.map_update)auto
+          qed
+        qed
+        then show ?thesis
+          by(simp add: one_it_def Some some Graph.digraph_abs_def Graph.neighbourhood_def neighbourhood_def)
+      qed
+    qed
+  qed
+
+
+  have "[foldr one_it xs BFS_tree]\<^sub>g = [BFS_tree]\<^sub>g \<union> {(u, v) |u v. u \<in> [frontier]\<^sub>s \<and> v \<in> neighbourhood [G]\<^sub>g u - [vis]\<^sub>s}"
+    using xs_prop(1) assms(2)
+  proof(induction xs arbitrary: frontier)
+    case Nil
+    then show ?case by simp
+  next
+    case (Cons a xs)
+    show ?case 
+    proof(cases "a \<in> set xs")
+      case True
+      have heper: "[foldr one_it xs BFS_tree]\<^sub>g \<union> {(a, v) |v. v \<in> neighbourhood [G]\<^sub>g a - [vis]\<^sub>s} =
+    [BFS_tree]\<^sub>g \<union> {(u, v). u \<in> [frontier]\<^sub>s \<and> v \<in> neighbourhood [G]\<^sub>g u \<and> v \<notin> [vis]\<^sub>s}"
+      using Cons.prems(1) True 
+      by (subst Cons(1)[of frontier])(auto simp add: Cons.prems(2))
+     show ?thesis 
+       using goal1_general heper 
+       by (auto simp add: one_it_graph_abs)
+   next
+     case False
+     have del_set:"[neighb_delete a frontier]\<^sub>s = set xs"
+       using Cons.prems(1) Cons.prems(2) False Graph.neighb.set.set_delete by auto
+     show ?thesis
+       using Cons.prems(1) Cons.prems(2) False Graph.neighb.set.set_delete 
+     by(auto simp add: one_it_graph_abs goal1_general Cons(1)[of "neighb_delete a frontier"] Cons.prems(2) Graph.neighb.set.invar_delete del_set sym[OF Cons(2)])
+ qed
+qed
+  thus "[expand_tree BFS_tree frontier vis]\<^sub>g =
+    [BFS_tree]\<^sub>g \<union> {(u, v) |u v. u \<in> [frontier]\<^sub>s \<and> v \<in> neighbourhood [G]\<^sub>g u - [vis]\<^sub>s}"
+    using xs_prop(2) by argo
+qed
+
+lemmas [code] = expand_tree_def next_frontier_def
+
+end
+
+fun fold_rbt where
+"fold_rbt f Leaf acc = acc"|
+"fold_rbt f (B l x r) acc= f x (fold_rbt f l (fold_rbt f r acc))"|
+"fold_rbt f (R l x r) acc= f x (fold_rbt f l (fold_rbt f r acc))"
+
+lemma fold_rbt_is_foldr_of_preorder:"fold_rbt f T acc = foldr f (map fst (preorder T)) acc "
+  by(induction f T acc arbitrary: rule: fold_rbt.induct) auto
 
 definition "t_set \<equiv> Tree2.set_tree"
 definition "neighb_inv \<equiv>  (\<lambda>t. (invc t \<and> invh t) \<and> Tree2.bst t)"
@@ -46,6 +386,50 @@ lemma Set2_satisfied: "Set2 neighb_empty neighb_delete isin t_set neighb_inv nei
   by(auto simp add: RBT_Set.empty_def neighb_empty_def neighb_delete_def t_set_def neighb_inv_def neighb_insert_def
                     neighb_union_def neighb_inter_def neighb_diff_def)
 
+definition "fold_neighb = (fold_rbt)"
+definition "fold_adj = (fold_rbt)"
+
+lemma prderorder_set:"set (map fst (preorder N)) = Tree2.set_tree N"
+  by(induction N rule: preorder.induct)auto
+
+lemma preorder_witness:"set (map fst (preorder N)) = t_set N \<and> fold_rbt f N acc = foldr f (map fst (preorder N)) acc"
+  unfolding fold_rbt_is_foldr_of_preorder prderorder_set t_set_def by auto
+
+lemma rbt_fold_spec:"neighb_inv N \<Longrightarrow> \<exists>xs. set xs = t_set N \<and> fold_rbt f N acc = foldr f xs acc"
+  using preorder_witness by metis
+
+lemma BFS_subprocedures_axioms: "BFS_subprocedures_axioms t_set neighb_inv fold_neighb fold_adj"
+ by(auto intro!: BFS_subprocedures_axioms.intro rbt_fold_spec
+           simp add: fold_neighb_def fold_adj_def )
+
+global_interpretation bfs_subprocedures: BFS_subprocedures
+where insert = neighb_insert 
+and sel = sel 
+and neighb_empty = neighb_empty 
+and diff = neighb_diff 
+and lookup = lookup 
+and empty = empty 
+and delete=delete 
+and isin = isin 
+and t_set=t_set
+and update=update 
+and adj_inv = M.invar
+and neighb_delete= neighb_delete
+and neighb_inv = neighb_inv 
+and union=neighb_union 
+and inter=neighb_inter 
+and fold_neighb = fold_neighb
+and fold_adj=fold_adj
+and G = G for G 
+defines next_frontier = bfs_subprocedures.next_frontier
+and expand_tree = bfs_subprocedures.expand_tree
+by(auto intro!: BFS_subprocedures.intro 
+           simp add: Pair_Graph_Specs_satisfied  Set2_satisfied BFS_subprocedures_axioms )
+
+lemma BFS_axioms:"BFS_axioms isin t_set M.invar \<emptyset>\<^sub>N neighb_inv lookup G (expand_tree G) (next_frontier G)"
+ by(fastforce intro!: BFS_axioms.intro 
+       simp add: bfs_subprocedures.expand_tree  bfs_subprocedures.next_frontier)
+
 global_interpretation bfs: BFS
 where insert = neighb_insert 
 and sel = sel 
@@ -62,9 +446,33 @@ and neighb_delete= neighb_delete
 and neighb_inv = neighb_inv 
 and union=neighb_union 
 and inter=neighb_inter 
-and G = F and t = "t::nat" and s = "s::nat"  for F t s
-defines  dfs_initial_state = dfs.initial_state 
-and neighbourhood=dfs.Graph.neighbourhood 
-and dfs_impl = dfs.DFS_impl
-  using Pair_Graph_Specs_satisfied Set2_satisfied 
-  by(auto intro!: DFS.intro)
+and expand_tree = "expand_tree G"
+and next_frontier = "next_frontier G"
+and G = G and srcs = srcs for G srcs
+defines bfs_initial_state = "bfs.initial_state"
+and bfs_impl = bfs.BFS_impl
+  by(auto intro!: BFS.intro simp add: Pair_Graph_Specs_satisfied Set2_satisfied BFS_axioms)
+
+definition "edges = [(0::nat, 1::nat), (0, 2), (2, 3), (2,4), (2,1), (1,5), (5,8), (8,7), (7,1),
+                     (7,2), (7,4), (4,3), (3,4), (3,3), (9, 8), (8, 1), (4,5), (5,10)]"
+
+definition "vertices = remdups (map prod.fst edges @ map prod.snd edges)"
+
+definition "nbs v = foldr (\<lambda> x tree. insert x tree) (remdups (map prod.snd (filter (\<lambda> e. prod.fst e = v) edges))) neighb_empty"
+
+definition "G = foldr (\<lambda> x tree. update x (nbs x) tree) vertices  empty"
+
+definition "src_list = [9::nat]"
+
+definition "srcs =  foldr (\<lambda> x tree. insert x tree) src_list empty"
+
+term bfs_initial_state
+term bfs_impl
+
+value edges
+value vertices
+value "neighb_diff (nbs 1) (nbs 2)"
+value G
+value "bfs_initial_state srcs"   
+value "bfs_impl G (bfs_initial_state srcs)"
+end
